testdata/modules/import_bare_pkgname_mismatch/cue.mod/module.cue
@@ -1,0 +1,2 @@
+module: "example.com/mm"
+language: version: "v0.16.1"
