testdata/modules/import_bare_pkgname_mismatch/foo/a.cue
@@ -1,0 +1,3 @@
+package bar
+
+Field: "v"
