testdata/modules/import_qualifier_pkgname_rescue/cue.mod/module.cue
@@ -1,0 +1,2 @@
+module: "example.com/qr"
+language: version: "v0.16.1"
