testdata/modules/import_qualifier_pkgname_rescue/main.cue
@@ -1,0 +1,5 @@
+package main
+
+import "example.com/qr/foo:bar"
+
+out: bar.Field
